code/hmac/Hacl.HMAC.fsti
@@ -1,0 +1,56 @@
+module Hacl.HMAC
+
+/// A generic, meta-programmed HMAC module. This one provides one concrete
+/// instantiation, namely HMAC-SHA2-256 instantiated with the HACL*
+/// implementation. In the future, this module may provide more implementations
+/// of HMAC, using optimized HACL versions of SHA2-256. For more algorithms, and
+/// for an assembly-optimized HMAC version that may call into Vale, see
+/// EverCrypt.HMAC.
+
+module B = Lib.Buffer
+module D = Hacl.Hash.Definitions
+
+open Spec.HMAC
+open Spec.Hash.Definitions
+open FStar.HyperStack.ST
+open Lib.Buffer
+open Lib.ByteBuffer
+open Lib.IntTypes
+
+#set-options "--max_fuel 0 --max_ifuel 0 --z3rlimit 20"
+
+let key_and_data_fits (a: hash_alg): Lemma
+  (ensures (block_length a + pow2 32 < max_input_length a))
+=
+  let open FStar.Integers in
+  assert_norm (8 * 16 + pow2 32 < pow2 61);
+  assert_norm (pow2 61 < pow2 125)
+
+inline_for_extraction
+let compute_st (a: hash_alg) =
+  tag: lbuffer uint8 (size (hash_length a)) ->
+  key: buffer uint8{ keysized a (B.length key) /\ B.disjoint key tag } ->
+  keylen: size_t{ v keylen = B.length key } ->
+  data: buffer uint8{ B.length data + block_length a < max_size_t } ->
+  datalen: size_t{ v datalen = B.length data } ->
+  Stack unit
+  (requires fun h0 -> B.live h0 tag /\ B.live h0 key /\ B.live h0 data)
+  (ensures fun h0 _ h1 -> modifies1 tag h0 h1 /\ (
+    assert_norm (pow2 32 < pow2 61 - 1);
+    assert_norm (pow2 32 < pow2 125 - 1);
+    B.as_seq h1 tag == hmac a
+      (B.as_seq #MUT #uint8 #keylen h0 key) (B.as_seq #MUT #uint8 #datalen h0 data)
+  ))
+
+inline_for_extraction noextract
+val mk_compute:
+  a: hash_alg ->
+  hash: D.hash_st a ->
+  alloca: D.alloca_st a ->
+  init: D.init_st a ->
+  update_multi: D.update_multi_st a ->
+  update_last: D.update_last_st a ->
+  finish: D.finish_st a ->
+  compute_st a
+
+val compute_sha2_256: compute_st SHA2_256
